

# SECTION-B

EASY

a) If  $z(x+y) = x^2 + y^2$ , show that  $\left(\frac{\partial z}{\partial x} - \frac{\partial z}{\partial y}\right)^2 = 4\left(1 - \frac{\partial z}{\partial x} - \frac{\partial z}{\partial y}\right)$

$$\star \left[ \frac{v \frac{\partial u}{\partial x} - u \frac{\partial v}{\partial x}}{v^2} \right] = \frac{d}{dx} \left( \frac{u}{v} \right) \rightarrow \frac{\partial z}{\partial x} = \frac{(x+y)(2x) - x^2 + y^2}{(x+y)^2}$$

$$z = \frac{x^2 + y^2}{x+y}$$

$$\rightarrow \frac{\partial z}{\partial x} = \frac{2x^2 + 2xy - x^2 + y^2}{(x+y)^2} \rightarrow \frac{\partial z}{\partial x} = \frac{x^2 + y^2 + 2xy}{(x+y)^2}$$

$$\rightarrow \frac{\partial z}{\partial y} = \frac{y^2 + x^2 + 2xy}{(x+y)^2}$$

$$\rightarrow \left[ \frac{\partial z}{\partial x} - \frac{\partial z}{\partial y} \right]^2 = \frac{x^2 - y^2 + 2xy - y^2 + x^2 - 2xy}{(x+y)^2}$$

$$\rightarrow \left( \frac{\partial z}{\partial x} - \frac{\partial z}{\partial y} \right)^2 = \frac{4(x-y)^2}{(x+y)^2}$$

$$\begin{aligned} \text{R.H.S.} & \rightarrow 4 \left( 1 - \left( \frac{x^2 + y^2 + 2xy}{(x+y)^2} \right) - \left( \frac{y^2 + x^2 + 2xy}{(x+y)^2} \right) \right) = 4 \left( \frac{x^2 + y^2 + 2xy}{(x+y)^2} - \frac{x^2 + y^2 + 2xy}{(x+y)^2} - \frac{y^2 + x^2 + 2xy}{(x+y)^2} \right) \\ & = 4 \left( \frac{x^2 + y^2 - 2xy}{(x+y)^2} \right) = 4 \frac{(x-y)^2}{(x+y)^2} \end{aligned}$$

Hence, L.H.S. = R.H.S.

b) let  $r^2 = x^2 + y^2 + z^2$  and  $v = r^m$ , p.t.  $V_{xx} + V_{yy} + V_{zz} = m(m+1)r^{m-2}$

$$r = \sqrt{x^2 + y^2 + z^2} \Rightarrow \frac{\partial r}{\partial x} = \frac{\partial \sqrt{x^2 + y^2 + z^2}}{\partial x} = \frac{1}{2} \cdot \frac{1}{\sqrt{x^2 + y^2 + z^2}} (2x)$$

$$V = r^m \Rightarrow V_x = m r^{m-1} \frac{\partial r}{\partial x} \quad \left[ \frac{\partial r}{\partial x} = \frac{x}{r} \right] \quad V_{xx} = m(m-1)r^{m-2} \frac{x^2}{r^2} + m r^{m-2}$$

$$\Rightarrow V_x = m r^{m-1} \left( \frac{x}{r} \right)$$

$$\Rightarrow V_x = m r^{m-2} x$$

$$\Rightarrow V_{xx} = x m(m-1) r^{m-3} \left( \frac{\partial r}{\partial x} \right) + r^{m-2} (1) m$$

$$= m \left[ x(m-1) r^{m-3} \left( \frac{x}{r} \right) + r^{m-2} \right]$$

$$\Rightarrow V_{yy} = m(m-1) y^2 r^{m-4} + m r^{m-2}$$

$$\Rightarrow V_{zz} = m(m-1) z^2 r^{m-4} + m r^{m-2}$$

$$\Rightarrow m(m-1) r^{m-4} (x^2 + y^2 + z^2) + 3m r^{m-2}$$

$$\Rightarrow m(m-1) r^{m-2} + 3m r^{m-2}$$

$$\Rightarrow m r^{m-2} (m+1)$$

Q. a) If  $u = \log(x^3 + y^3 + z^3 - 3xyz)$  then  $\left(\frac{\partial}{\partial x} + \frac{\partial}{\partial y} + \frac{\partial}{\partial z}\right)^2 u$

$$= -9$$

Let  $\left(\frac{\partial}{\partial x} + \frac{\partial}{\partial y} + \frac{\partial}{\partial z}\right)^2 u = \left(\frac{\partial}{\partial x} + \frac{\partial}{\partial y} + \frac{\partial}{\partial z}\right) \cdot \left(\frac{\partial u}{\partial x} + \frac{\partial u}{\partial y} + \frac{\partial u}{\partial z}\right)$

$\Rightarrow \frac{\partial u}{\partial x} = \frac{3x^2 - 3yz}{x^3 + y^3 + z^3 - 3xyz}$  similarly,  $\frac{\partial u}{\partial y} = \frac{3y^2 - 3xz}{x^3 + y^3 + z^3 - 3xyz}$

$\Rightarrow \frac{\partial u}{\partial z} = \frac{3z^2 - 3xy}{x^3 + y^3 + z^3 - 3xyz}$

$\Rightarrow \left(\frac{\partial}{\partial x} + \frac{\partial}{\partial y} + \frac{\partial}{\partial z}\right)^2 u = \left(\frac{\partial}{\partial x} + \frac{\partial}{\partial y} + \frac{\partial}{\partial z}\right) \cdot \left(\frac{3x^2 - 3yz}{x^3 + y^3 + z^3 - 3xyz} + \frac{3y^2 - 3xz}{x^3 + y^3 + z^3 - 3xyz} + \frac{3z^2 - 3xy}{x^3 + y^3 + z^3 - 3xyz}\right)$

[d]  $a^3 + b^3 + c^3 - 3abc = (a+b+c)(a^2 + b^2 + c^2 - ab - bc - ca)$

$\Rightarrow 3 \left(\frac{\partial}{\partial x} + \frac{\partial}{\partial y} + \frac{\partial}{\partial z}\right) \cdot \left(\frac{1}{x+y+z}\right) = 3 \left(\frac{\partial}{\partial x} \left(\frac{1}{x+y+z}\right) + \frac{\partial}{\partial y} \left(\frac{1}{x+y+z}\right) + \frac{\partial}{\partial z} \left(\frac{1}{x+y+z}\right)\right)$

$= 3 \left[ -1(x+y+z)^{-2} (1+1+1) + \dots \right] = -\frac{9}{(x+y+z)^2}$

$= 3 \left[ \frac{-1}{(x+y+z)^2} - \frac{1}{(x+y+z)^2} - \frac{1}{(x+y+z)^2} \right] = -\frac{9}{(x+y+z)^2}$

b) If  $v = x^y y^x$ , prove that  $x \frac{\partial v}{\partial x} + y \frac{\partial v}{\partial y} = v(x+y+\log v)$

$\log v = \log x^y y^x$

$\log v = \log x^y + \log y^x$

$\Rightarrow \log v = y \log x + x \log y$

$\Rightarrow$  diff. w.r.t.  $x$  partially, we get

$\frac{1}{v} \frac{\partial v}{\partial x} = y \left(\frac{1}{x}\right) + \log y$

$\frac{\partial v}{\partial x} = v \cdot y + v \log y$

Teacher's Signature \_\_\_\_\_

Partially diff. ① w.r.t  $y$ , we get

$$\frac{1}{v} \cdot \frac{\partial v}{\partial y} = v(\log x) + x \frac{1}{y}$$

$$\frac{\partial v}{\partial y} = v \log x + v \cdot \frac{x}{y}$$

$$\Rightarrow x \cdot \frac{\partial x}{\partial x} + y \frac{\partial y}{\partial y} = x(v \cdot y + v \log x) + y(v \log x + v \cdot \frac{x}{y})$$

$$= v \cdot y + vx \log y + vy \log x + vx$$

$$= v [x + y + (x \log y + y \log x)]$$

$$= v [x + y + \log v]$$

hence, L.H.S = R.H.S

a) If  $u = \sin^{-1}(x-y)$ ,  $x = 3t$  and  $y = 4t^3$ , s.t.  $\frac{\partial u}{\partial t} = \frac{3}{\sqrt{1-t^2}}$

$$\frac{\partial u}{\partial t} = \frac{\partial u}{\partial x} \cdot \frac{\partial x}{\partial t} + \frac{\partial u}{\partial y} \cdot \frac{\partial y}{\partial t} = \frac{1}{\sqrt{1-(x-y)^2}} \cdot (3) + \frac{1}{\sqrt{1-(x-y)^2}} (12t^2)$$

$$\frac{\partial u}{\partial x} = \frac{1}{\sqrt{1-x-y^2}}$$

$$\frac{\partial u}{\partial t} = \frac{3[1-4t^2]}{\sqrt{1-16t^6+24t^4-9t^2}}$$

$$\frac{\partial u}{\partial t} = 3$$

$$\frac{\partial u}{\partial t} = \frac{3(1-4t^2)}{\sqrt{(1-t)(1-4t^2)^2}} = \frac{3}{\sqrt{1-t}}$$

$$\frac{\partial u}{\partial y} = \frac{-1}{\sqrt{1-x-y^2}}$$

$$\frac{\partial y}{\partial t} = 12t^2$$

3) If  $u = x^2 + y^2 + z^2$  and  $x = e^{3t}$ ,  $y = e^{3t} \sin 3t$ ,  $z = e^{3t} \cos 3t$   
Find  $\frac{du}{dt}$  as a total derivative

$$\frac{du}{dt} = \frac{\partial u}{\partial x} \cdot \frac{dx}{dt} + \frac{\partial u}{\partial y} \cdot \frac{dy}{dt} + \frac{\partial u}{\partial z} \cdot \frac{dz}{dt}$$

$$\frac{\partial u}{\partial x} = 2x; \frac{\partial u}{\partial t} = 2e^{3t}; \frac{\partial u}{\partial y} = 2y; \frac{dy}{dt} = e^{3t}(3\cos 3t + \sin 3t)$$

$$\frac{dz}{dt} = e^{3t}(-3\sin 3t + \cos 3t); \frac{\partial u}{\partial z} = 2z = 2e^{3t} \cos 3t$$

$$\frac{du}{dt} = 2x(2e^{3t}) + 2y(e^{3t}(3\cos 3t + \sin 3t)) + 2z(e^{3t}(-3\sin 3t + \cos 3t))$$

$$= 2(e^{3t})(2e^{3t}) + 2(e^{3t} \sin 3t)(2e^{3t}(3\cos 3t + \sin 3t)) + 2(e^{3t} \cos 3t)(e^{3t}(-3\sin 3t + \cos 3t))$$

$$= 4e^{6t} + 4e^{6t} \sin^2 3t - 6e^{6t} \sin 3t \cos 3t + 4e^{6t} \cos^2 3t$$

$$\frac{du}{dt} = 8e^{6t}$$

⇒ MODERATE

Q. By the substitution,  $u = x^2 - y^2$ ,  $v = 2xy$ ,  $f(x, y) = \theta(u, v)$ .  
S.T.  $\frac{\partial^2 f}{\partial x^2} + \frac{\partial^2 f}{\partial y^2} = a(x^2 + y^2) \left( \frac{\partial^2 \theta}{\partial u^2} + \frac{\partial^2 \theta}{\partial v^2} \right)$

A) Now,  $\frac{\partial f}{\partial x} = \frac{\partial \theta}{\partial u} \cdot \frac{\partial u}{\partial x} + \frac{\partial \theta}{\partial v} \cdot \frac{\partial v}{\partial x}$

$$\Rightarrow \frac{\partial f}{\partial x} = \frac{\partial \theta}{\partial u} (2x) + \frac{\partial \theta}{\partial v} (2y) \Rightarrow \frac{\partial}{\partial x} \left[ \frac{\partial \theta}{\partial u} + \frac{\partial \theta}{\partial v} \right]$$

$$\Rightarrow \frac{\partial^2 f}{\partial x^2} = \frac{\partial}{\partial x} \left[ \frac{\partial f}{\partial x} \right] = \left[ 2x \frac{\partial}{\partial u} + 2y \frac{\partial}{\partial v} \right] \left[ \frac{\partial \theta}{\partial u} + \frac{\partial \theta}{\partial v} \right]$$

Teacher's Signature

$$\frac{\partial^2 f}{\partial u^2} = 4x^2 \frac{\partial^2 \theta}{\partial u^2} + 4xy \frac{\partial^2 \theta}{\partial u \partial v} + 4y^2 \frac{\partial^2 \theta}{\partial v^2} //$$

$$\frac{\partial^2 f}{\partial u^2} = 4x^2 \frac{\partial^2 \theta}{\partial u^2} + 8xy \frac{\partial^2 \theta}{\partial u \partial v} + 4y^2 \frac{\partial^2 \theta}{\partial v^2} \quad \text{--- (1)}$$

Similarly,  $\frac{\partial f}{\partial y} = \frac{\partial \theta}{\partial y}$

$$\frac{\partial f}{\partial y} = \frac{\partial \theta}{\partial u} \cdot \frac{\partial u}{\partial y} + \frac{\partial \theta}{\partial v} \cdot \frac{\partial v}{\partial y} = \frac{\partial \theta}{\partial u} \cdot (-xy) + \frac{\partial \theta}{\partial v} (2x)$$

$$\Rightarrow \frac{\partial}{\partial y} = -xy \frac{\partial}{\partial u} + 2x \frac{\partial}{\partial v} \quad \text{--- (2)} \quad \frac{\partial^2 f}{\partial y^2} = \frac{\partial}{\partial y} \left[ \frac{\partial f}{\partial y} \right]$$

$$\Rightarrow \frac{\partial^2 f}{\partial y^2} = \left[ -xy \frac{\partial}{\partial u} + 2x \frac{\partial}{\partial v} \right] \left[ -xy \frac{\partial \theta}{\partial u} + 2x \frac{\partial \theta}{\partial v} \right]$$

$$\Rightarrow \frac{\partial^2 f}{\partial y^2} = 4y^2 \frac{\partial^2 \theta}{\partial u^2} - 4xy \frac{\partial^2 \theta}{\partial u \partial v} - 4xy \frac{\partial^2 \theta}{\partial u \partial v} + 4x^2 \frac{\partial^2 \theta}{\partial v^2}$$

$$\Rightarrow \frac{\partial^2 f}{\partial y^2} = 4x^2 \frac{\partial^2 \theta}{\partial v^2} - 8xy \frac{\partial^2 \theta}{\partial u \partial v} + 4y^2 \frac{\partial^2 \theta}{\partial u^2} \quad \text{--- (2)}$$

(i) L.H.S  $\frac{\partial^2 f}{\partial x^2} + \frac{\partial^2 f}{\partial y^2} = 4x^2 \frac{\partial^2 \theta}{\partial u^2} + 8xy \frac{\partial^2 \theta}{\partial u \partial v} + 4y^2 \frac{\partial^2 \theta}{\partial v^2}$

$$= 4(x^2 + y^2) \left[ \frac{\partial^2 \theta}{\partial u^2} + \frac{\partial^2 \theta}{\partial v^2} \right] + 4x^2 \frac{\partial^2 \theta}{\partial v^2} - 8xy \frac{\partial^2 \theta}{\partial u \partial v} + 4y^2 \frac{\partial^2 \theta}{\partial u^2}$$

L.H.S = R.H.S

Hence Proved

Q. 1) If  $x = r \cos \theta$ ,  $y = r \sin \theta$  evaluate  $\frac{\partial(x,y)}{\partial(r,\theta)}$ ,  $\frac{\partial(x,y)}{\partial(r,\theta)}$  S.P.T

Given

$$\frac{\partial(x,y)}{\partial(r,\theta)} = \begin{vmatrix} \frac{\partial x}{\partial r} & \frac{\partial x}{\partial \theta} \\ \frac{\partial y}{\partial r} & \frac{\partial y}{\partial \theta} \end{vmatrix} \Rightarrow x = r \cos \theta \Rightarrow y = r \sin \theta$$

$$\Rightarrow \cos \theta = \frac{x}{r} \Rightarrow \sin \theta = \frac{y}{r}$$

$$\Rightarrow r = \sqrt{x^2 + y^2}$$

$$\Rightarrow \frac{\partial x}{\partial r} = \frac{\partial}{\partial r} (r \cos \theta) = \cos \theta = \frac{x}{r}$$

$$\frac{\partial x}{\partial \theta} = -r \sin \theta = -y$$

$$\frac{\partial y}{\partial r} = \sin \theta = \frac{y}{r}$$

$$\frac{\partial y}{\partial \theta} = r \cos \theta = x$$

Given,  $x = r \cos \theta$ ,  $y = r \sin \theta$

$$\frac{y}{x} = \tan \theta \Rightarrow \theta = \tan^{-1} \frac{y}{x}$$

$$\frac{\partial \theta}{\partial x} = \frac{1}{1 + \frac{y^2}{x^2}} \left( -\frac{y}{x^2} \right) \Rightarrow \frac{\partial \theta}{\partial x} = \frac{-y}{x^2 + y^2}$$

$$\frac{\partial \theta}{\partial y} = \frac{1}{1 + \frac{y^2}{x^2}} \left( \frac{1}{x} \right) \Rightarrow \frac{\partial \theta}{\partial y} = \frac{x}{x^2 + y^2}$$

$$\frac{\partial \theta}{\partial x} = \frac{-y}{x^2 + y^2} \quad \frac{\partial \theta}{\partial y} = \frac{x}{x^2 + y^2}$$

$$\Rightarrow \begin{vmatrix} \frac{\partial x}{\partial r} & \frac{\partial x}{\partial \theta} \\ \frac{\partial y}{\partial r} & \frac{\partial y}{\partial \theta} \end{vmatrix} = \begin{vmatrix} \frac{x}{r} & -y \\ \frac{y}{r} & x \end{vmatrix} = \frac{x^2}{r^2} + \frac{y^2}{r^2} = \frac{x^2 + y^2}{r^2} = \frac{r^2}{r^2} = 1$$

$$\Rightarrow \frac{\partial(x,y)}{\partial(r,\theta)} = \begin{vmatrix} \frac{\partial x}{\partial r} & \frac{\partial x}{\partial \theta} \\ \frac{\partial y}{\partial r} & \frac{\partial y}{\partial \theta} \end{vmatrix} = \begin{vmatrix} \cos \theta & -r \sin \theta \\ \sin \theta & r \cos \theta \end{vmatrix} = r$$

$$\Rightarrow \frac{1}{r} \cdot r = 1 //$$

Hence Proved,

b) a) If  $u = x^2 - 2y^2$ ,  $v = 2x^2 - y^2$  where  $x = r \cos \theta$ ,  $y = r \sin \theta$ ,

$$\text{S.T } \frac{\partial(u,v)}{\partial(r,\theta)} = 6r^3 \sin 2\theta$$

$$\text{A) } \frac{\partial(u,v)}{\partial(x,\theta)} = \frac{\partial(u,v)}{\partial(x,y)} \cdot \frac{\partial(x,y)}{\partial(r,\theta)} = \begin{vmatrix} \frac{\partial u}{\partial x} & \frac{\partial u}{\partial y} \\ \frac{\partial v}{\partial x} & \frac{\partial v}{\partial y} \end{vmatrix} \cdot \begin{vmatrix} \frac{\partial x}{\partial r} & \frac{\partial x}{\partial \theta} \\ \frac{\partial y}{\partial r} & \frac{\partial y}{\partial \theta} \end{vmatrix}$$

$$u, v \begin{matrix} \nearrow x \\ \searrow y \end{matrix} \begin{matrix} \nearrow r, \theta \\ \searrow \end{matrix} = \begin{vmatrix} 2x & -2y \\ 4x & -y \end{vmatrix} \cdot \begin{vmatrix} \cos \theta & -r \sin \theta \\ \sin \theta & r \cos \theta \end{vmatrix}$$

$$= (4xy + 16xy)(r)$$

$$= 12xyr = 12(r \cos \theta)(r \sin \theta)$$

$$\rightarrow 12r^2 \sin \theta \cos \theta = \underline{\underline{6r^3 \sin 2\theta}}$$

3) a) If  $u = xyz$ ,  $v = x^2 + y^2 + z^2$ ,  $w = x + y + z$ , find  $\frac{\partial(x,y,z)}{\partial(u,v,w)}$

$$\text{A) } \frac{\partial(x,y,z)}{\partial(u,v,w)} = \begin{vmatrix} \frac{\partial x}{\partial u} & \frac{\partial x}{\partial v} & \frac{\partial x}{\partial w} \\ \frac{\partial y}{\partial u} & \frac{\partial y}{\partial v} & \frac{\partial y}{\partial w} \\ \frac{\partial z}{\partial u} & \frac{\partial z}{\partial v} & \frac{\partial z}{\partial w} \end{vmatrix} \Rightarrow \frac{\partial(x,y,z)}{\partial(u,v,w)} \cdot \frac{\partial(u,v,w)}{\partial(x,y,z)} = 1$$

$$\frac{\partial(u,v,w)}{\partial(x,y,z)} = \begin{vmatrix} \frac{\partial u}{\partial x} & \frac{\partial u}{\partial y} & \frac{\partial u}{\partial z} \\ \frac{\partial v}{\partial x} & \frac{\partial v}{\partial y} & \frac{\partial v}{\partial z} \\ \frac{\partial w}{\partial x} & \frac{\partial w}{\partial y} & \frac{\partial w}{\partial z} \end{vmatrix} = \begin{vmatrix} yz & xz & xy \\ 2x & 2y & 2z \\ 1 & 1 & 1 \end{vmatrix}$$

$$\begin{aligned}
 & yz(2y-2z) - xz(2x-2z) + xy(2x-2y) \\
 & 2y^2z - 2yz^2 - 2x^2z + 2xz^2 + 2x^2y - 2xy^2 \\
 & = 2(y^2z - yz^2 - x^2z + xz^2 + x^2y - xy^2)
 \end{aligned}$$

$$\therefore \frac{\partial(x, y, z)}{\partial(u, v, w)} = \frac{1}{2(y^2z - yz^2 - x^2z + xz^2 + x^2y - xy^2)}$$

Q. If  $u = \frac{x+y}{1-xy}$ ,  $v = \tan^{-1}x + \tan^{-1}y$ , find  $\frac{\partial(u,v)}{\partial(x,y)}$ . Are  $u$  and  $v$  functionally related? If  $u$ , find the relation.

Ans. If  $J\left(\frac{u,v}{(x,y)}\right) = 0$ , then functionally dependant.

$$\frac{\partial u}{\partial x} = \frac{1-xy(1) - x+y(1)}{(1-xy)^2} = \frac{1-xy+x+y}{(1-xy)^2} = \frac{1+y^2}{(1-xy)^2}$$

$$\frac{\partial u}{\partial y} = \frac{1+x^2}{1-xy^2} // \quad ; \quad \frac{\partial v}{\partial x} = \frac{1}{1+x^2} \quad ; \quad \frac{\partial v}{\partial y} = \frac{1}{1+y^2}$$

$$\Rightarrow \begin{vmatrix} \frac{\partial u}{\partial x} & \frac{\partial u}{\partial y} \\ \frac{\partial v}{\partial x} & \frac{\partial v}{\partial y} \end{vmatrix} = 0 // \quad * \text{ So functionally dependant }$$

$$\begin{aligned}
 \rightarrow \text{Relation} \rightarrow u &= \frac{x+y}{1-xy} \quad ; \quad v = \tan^{-1}x + \tan^{-1}y \\
 \rightarrow v &= \tan^{-1}u \\
 &= \tan^{-1}\left(\frac{x+y}{1-xy}\right) = \tan^{-1}x
 \end{aligned}$$



6xy^2 - 12x^2y^2 - 6xy^3 TYPICAL f(x,y) = x^3y^2(1-x-y)

① Discuss maxima & minima of f(x,y) = x^3y^2(1-x-y)

② f(x,y) = x^3y^2 - 2x^4y^2 - x^3y^3

$$\frac{\partial f}{\partial x} = 3x^2y^2 - 4x^3y^2 - 3x^2y^3 = 0 \Rightarrow x^2y^2(3-4x-3y) = 0$$

$$\frac{\partial f}{\partial y} = x^3(2y - 2yx - 3y^2) = 0 \Rightarrow x^3y(2-2x-3y) = 0$$

$\Rightarrow x=0, y=0 \Rightarrow (0,0)$  ;  $4x+3y=3$   
 $2x+3y=2$   
 $x=\frac{1}{2}, y=\frac{1}{3}$

\*  $(x,y) = (\frac{1}{2}, \frac{1}{3})$

Now, partially diff ② & ③ w.r.t x & y

$\frac{\partial^2 f}{\partial x^2} = r = 6xy^2 - 12x^2y^2 - 6xy^3 = 6xy^2(1-2x-y)$

$\frac{\partial^2 f}{\partial y^2} = t = 2x^3(1-x-2y)$  ;  $\frac{\partial^2 f}{\partial x \partial y} = s = x^2y(6-8x-9y)$

Now, at point  $(\frac{1}{2}, \frac{1}{3}) \Rightarrow r = -\frac{1}{9}, t = -\frac{1}{2}, s = -\frac{1}{2}$

at  $rt - s^2 > 0$ , check  $r = -\frac{1}{9} < 0$

So,  $(\frac{1}{2}, \frac{1}{3})$  is point of maxima //

③ Discuss the maxima & minima of f(x,y) = x^3 + y^3 - 3axy

①  $\frac{\partial f}{\partial x} = 3x^2 - 3ay = 0$  ;  $\frac{\partial f}{\partial y} = 3y^2 - 3ax = 0$

$x^2 = ay$  ;  $y^2 = ax \Rightarrow (x,y) = (0,0) \text{ \& } (a,a)$

$y = \frac{x^2}{a} \Rightarrow (\frac{x^2}{a})^2 = ax \Rightarrow \text{At point } (a,a)$

Now, partially diff eq ① & ② further

$\frac{\partial^2 f}{\partial x^2} = 6x = r \Rightarrow \frac{\partial^2 f}{\partial y^2} = 6y = t$

$\frac{\partial^2 f}{\partial x \partial y} = -3a = s$  Now,  $rt - s^2 = 36xy - 9a^2$

\* At Point (0,0),  $rt - s^2 = -9a^2 < 0$

as  $rt - s^2 < 0$ , saddle point = (0,0)

at  $rt - s^2 > 0$ , check  $r$

$r = 6x = 6a > 0 \Rightarrow r > 0$  (point of minima)

\* (a,a) is point of minima

2) Find the volume of the greatest rectangular parallelepiped that can be inscribed in ellipsoid  $\frac{x^2}{a^2} + \frac{y^2}{b^2} + \frac{z^2}{c^2} = 1$

Given,  $\frac{x^2}{a^2} + \frac{y^2}{b^2} + \frac{z^2}{c^2} = 1$

Let,  $f(x, y, z) = 8xyz$  [objective function]

$g(x, y, z) = \frac{x^2}{a^2} + \frac{y^2}{b^2} + \frac{z^2}{c^2} - 1$  [constraint function]

$F(x, y, z) = f(x, y, z) + \lambda g(x, y, z)$

$F(x, y, z) = 8xyz + \lambda \left( \frac{x^2}{a^2} + \frac{y^2}{b^2} + \frac{z^2}{c^2} - 1 \right)$

$\frac{\partial F}{\partial x} = 0 \Rightarrow 8yz + \lambda \left( \frac{2x}{a^2} \right) = 0 \Rightarrow \frac{4yz a^2}{x} = -\lambda$

Similarly  $\frac{\partial F}{\partial y} = 0 \Rightarrow \frac{4zx b^2}{y} = -\lambda$  and  $\frac{\partial F}{\partial z} = 0 \Rightarrow \frac{4xy c^2}{z} = -\lambda$

$\frac{4yz a^2}{x} = \frac{4zx b^2}{y} = \frac{4xy c^2}{z} = -\lambda$

$\frac{yz a^2}{x} = \frac{zx b^2}{y}$

$\frac{z}{y} a^2 = \frac{x}{y} b^2$

$y^2 a^2 = x^2 b^2$

$\frac{y^2}{b^2} = \frac{x^2}{a^2}$

$\frac{y}{b} = \frac{x}{a}$

$\frac{x^2}{a^2} + \frac{y^2}{b^2} + \frac{z^2}{c^2} = 1$

$\frac{3x^2}{a^2} = 1$

$x = \frac{a}{\sqrt{3}}$

$y = \frac{b}{\sqrt{3}}$

$z = \frac{c}{\sqrt{3}}$

Required volume  $= 8xyz = \frac{8abc}{3\sqrt{3}}$

2) a) Find the dimensions of the rectangular box, open at the top, of maximum capacity whose surface is 432 sq. units.

b) let  $x, y, z$  be the dimensions of rectangular box.  
 Volume =  $V = xyz$ ; Total surface area =  $2xy + 2yz + 2xz$  but box is open at top  
 $\Rightarrow xy + 2yz + 2xz = 432$

$$F = xyz + \lambda(xy + 2yz + 2xz - 432)$$

$$F_x = 0 \Rightarrow yz + \lambda(y + 2z) = 0 \Rightarrow yz = -\lambda(y + 2z)$$

$$F_y = 0 \Rightarrow xz + \lambda(x + 2z) = 0 \Rightarrow xz = -\lambda(x + 2z)$$

$$F_z = 0 \Rightarrow xy + \lambda(2y + 2x) = 0 \Rightarrow xy = -\lambda(2x + 2y)$$

$$\Rightarrow \frac{y}{x} = \frac{y + 2z}{x + 2z} \Rightarrow \underline{x = y} \Rightarrow \frac{z}{y} = \frac{x + 2z}{2x + 2y} \Rightarrow y = \underline{2z}$$

$$\text{So, } xy + 2xz + 2zy = 432 \Rightarrow 4z^2 + 4z^2 + 4z^2 = 432$$

$$\Rightarrow z = 6 \Rightarrow x = 12, y = 12 \text{ The dimensions are } \underline{(12, 12, 6)}$$

c) The sum of 3 no's is constant. P.T their product is max when they are equal.

Given,  $x + y + z = b \Rightarrow x + y + z - b = 0$  & product is  $P = xyz$  should be max.

Here, objective function :-  $f(x, y, z) = xyz$

constrained function :-  $\phi(x, y, z) = x + y + z - b$

$$* F(x, y, z) = f(x, y, z) + \lambda \phi(x, y, z) \Rightarrow F(x, y, z) = xyz + \lambda(x + y + z - b)$$

$$* \frac{\partial F}{\partial x} = yz + \lambda = 0 \quad * \frac{\partial F}{\partial y} = xz + \lambda = 0 \quad * \frac{\partial F}{\partial z} = xy + \lambda = 0$$

$$\lambda = -yz \quad \lambda = -xz \quad \lambda = -xy$$

$$\Rightarrow x = y = z \quad * x + x + x = b \text{ so } \left(\frac{b}{3}, \frac{b}{3}, \frac{b}{3}\right) \Rightarrow x = \frac{b}{3} = y = z$$

$$* \text{max value} = \frac{b^3}{27}$$